lib/Lib.Buffer.fsti
@@ -144,6 +144,18 @@ val modifies_sub: #t:buftype -> #a:Type0 -> #len:size_t -> b:lbuffer_t t a len
     (ensures  modifies (loc b) h0 h1)
     [SMTPat (modifies (loc (gsub b start n)) h0 h1)]
 
+val modifies1_is_modifies2: #a0:Type0 -> #a1:Type0 ->
+  b0:buffer_t MUT a0 -> b1:buffer_t MUT a1 -> h0: HS.mem -> h1: HS.mem ->
+  Lemma
+  (requires (live h0 b0 /\ live h0 b1))
+  (ensures  (modifies1 b0 h0 h1 ==> modifies2 b0 b1 h0 h1))
+
+val modifies1_is_modifies3: #a0:Type0 -> #a1:Type0 -> #a2:Type0 ->
+  b0:buffer_t MUT a0 -> b1:buffer_t MUT a1 -> b2:buffer_t MUT a2 -> h0: HS.mem -> h1: HS.mem ->
+  Lemma
+  (requires (live h0 b0 /\ live h0 b1 /\ live h0 b2))
+  (ensures  (modifies1 b0 h0 h1 ==> modifies3 b0 b1 b2 h0 h1))
+
 inline_for_extraction
 val as_seq_gsub:
     #t:buftype
@@ -447,6 +459,27 @@ val loop_nospec2:
   Stack unit
     (requires fun h -> h0 == h /\ live h0 buf1 /\ live h0 buf2)
     (ensures  fun _ _ h1 -> modifies2 buf1 buf2 h0 h1)
+
+(** Loop combinator with just memory safety specification *)
+inline_for_extraction noextract
+val loop_nospec3:
+    #h0:mem
+  -> #a1:Type0
+  -> #a2:Type0
+  -> #a3:Type0
+  -> #len1:size_t
+  -> #len2:size_t
+  -> #len3:size_t
+  -> n:size_t
+  -> buf1:lbuffer a1 len1
+  -> buf2:lbuffer a2 len2
+  -> buf3:lbuffer a3 len3
+  -> impl: (i:size_t{v i < v n} -> Stack unit
+      (requires fun h -> modifies3 buf1 buf2 buf3 h0 h)
+      (ensures  fun _ _ h1 -> modifies3 buf1 buf2 buf3 h0 h1)) ->
+  Stack unit
+    (requires fun h -> h0 == h /\ live h0 buf1 /\ live h0 buf2 /\ live h0 buf3)
+    (ensures  fun _ _ h1 -> modifies3 buf1 buf2 buf3 h0 h1)
 
 (** Loop combinator with just memory safety specification *)
 inline_for_extraction noextract
